tests/Instantiate.v
@@ -1,0 +1,72 @@
+(****************************************************************************)
+(* Copyright 2020 The Project Oak Authors                                   *)
+(*                                                                          *)
+(* Licensed under the Apache License, Version 2.0 (the "License")           *)
+(* you may not use this file except in compliance with the License.         *)
+(* You may obtain a copy of the License at                                  *)
+(*                                                                          *)
+(*     http://www.apache.org/licenses/LICENSE-2.0                           *)
+(*                                                                          *)
+(* Unless required by applicable law or agreed to in writing, software      *)
+(* distributed under the License is distributed on an "AS IS" BASIS,        *)
+(* WITHOUT WARRANTIES OR CONDITIONS OF ANY KIND, either express or implied. *)
+(* See the License for the specific language governing permissions and      *)
+(* limitations under the License.                                           *)
+(****************************************************************************)
+
+Require Import Program.Basics.
+From Coq Require Import Bool.Bool.
+From Coq Require Import Ascii String.
+From Coq Require Import Lists.List.
+From Coq Require Import ZArith.
+Import ListNotations.
+
+Require Import Cava.Cava.
+Require Import Cava.Monad.CavaMonad.
+
+Local Open Scope list_scope.
+Local Open Scope monad_scope.
+Local Open Scope string_scope.
+
+(* NAND gate example. Fist, let's define an overloaded NAND gate
+   description. *)
+
+Definition nand2Interface
+  := combinationalInterface
+     "nand2"
+     (mkPort "a" Bit, mkPort "b" Bit)
+     (mkPort "c" Bit)
+     [].
+
+
+Definition nand2_gate {m bit} `{Cava m bit} (ab : bit * bit) : m bit :=
+  x <- and2 ab ;;
+  inv x.
+
+Definition nand3Interface
+  := combinationalInterface
+     "instantiate"
+     (mkPort "a" Bit, mkPort "b" Bit, mkPort "c" Bit)
+     (mkPort "d" Bit)
+     [].
+
+Definition nand3_gate {m bit} `{cava : Cava m bit} '(a, b, c) :=
+    n1 <- instantiate nand2Interface nand2_gate (a, b) ;;
+    instantiate nand2Interface nand2_gate (c, n1).   
+
+Definition instantiateNetlist := makeNetlist nand3Interface nand3_gate.
+
+(* Test bench tables for generated SystemVerilog simulation test bench *)
+Definition instantiate_tb_inputs : list (bool * bool * bool) :=
+ [(false, false, false);
+  (false, true, false);
+  (true, false, true);
+  (true, true, true)].
+
+(* Compute expected outputs. *)
+Definition instantiate_tb_expected_outputs : list bool :=
+  map (fun i => combinational (nand3_gate i)) instantiate_tb_inputs.
+
+Definition instantiate_tb :=
+  testBench "instantiate_tb" nand3Interface instantiate_tb_inputs instantiate_tb_expected_outputs.
+
